fix: def -> theorem

Algebra/Reflection/CommGroup.lean
@@ -253,7 +253,7 @@ class Reflect {α} (s : GroupSig α) (x : α) (xs : List α) where
   expr : Expr xs
   eval_eq : expr.eval s = x
 
-protected def Reflect.eq {α} (s : GroupSig α) (x xs) [inst : Reflect s x xs] : inst.expr.eval s = x := inst.eval_eq
+protected theorem Reflect.eq {α} (s : GroupSig α) (x xs) [inst : Reflect s x xs] : inst.expr.eval s = x := inst.eval_eq
 
 namespace Reflect
 variable {α} (s : GroupSig α) [CommGroup s]
