Extra/Nat/NeZero.lean
@@ -7,11 +7,11 @@ import Extra.Nat.Lemmas
 
 namespace Nat
 
-def ne_zero (n : Nat) [self : NeZero n] : n ≠ 0 := self.out
+theorem ne_zero (n : Nat) [self : NeZero n] : n ≠ 0 := self.out
 
-def zero_ne (n : Nat) [self : NeZero n] : 0 ≠ n := self.out.symm
+theorem zero_ne (n : Nat) [self : NeZero n] : 0 ≠ n := self.out.symm
 
-def zero_lt (n : Nat) [self : NeZero n] : 0 < n := Nat.zero_lt_of_ne_zero <| ne_zero n
+theorem zero_lt (n : Nat) [self : NeZero n] : 0 < n := Nat.zero_lt_of_ne_zero <| ne_zero n
 
 instance (n : Nat) : NeZero (n ^ 0) where
   out := Nat.one_ne_zero
