Logic/Relation/Classes.lean
@@ -63,7 +63,7 @@ instance {α} (r : α → α → Prop) [Symmetric r] : HSymmetric r r := ⟨Symm
 
 abbrev Asymmetric (r : α → α → Prop) := HSymmetric r (¬r . .)
 
-protected def Asymmetric.asymm {α} {r : α → α → Prop} [Asymmetric r] {x y : α} : r x y → ¬r y x := HSymmetric.symm (r:=r) (s:=(¬r . .))
+protected theorem Asymmetric.asymm {α} {r : α → α → Prop} [Asymmetric r] {x y : α} : r x y → ¬r y x := HSymmetric.symm (r:=r) (s:=(¬r . .))
 
 instance (α) : Symmetric (α:=α) (.=.) := ⟨Eq.symm⟩
 instance (α) : Symmetric (α:=α) (.≠.) := ⟨Ne.symm⟩
@@ -161,12 +161,10 @@ instance [Reflexive r] [Euclidean r] : Symmetric r where
 instance [Symmetric r] [Transitive r] : Euclidean r where
   eucl hxy hxz := Transitive.trans (Symmetric.symm hxy) hxz
 
-@[implicit_reducible]
-def Euclidean.toSymmetric {α} (r : α → α → Prop) [Reflexive r] [Euclidean r] : Symmetric r where
+theorem Euclidean.toSymmetric {α} (r : α → α → Prop) [Reflexive r] [Euclidean r] : Symmetric r where
   symm hxy := Euclidean.eucl hxy Reflexive.rfl
 
-@[implicit_reducible]
-def Euclidean.toTransitive {α} (r : α → α → Prop) [Symmetric r] [Euclidean r] : Transitive r where
+theorem Euclidean.toTransitive {α} (r : α → α → Prop) [Symmetric r] [Euclidean r] : Transitive r where
   trans hxy hyz := Euclidean.eucl (Symmetric.symm hxy) hyz
 
 /-! ## Totality -/
@@ -191,8 +189,7 @@ class Comparison {α} (r : α → α → Prop) : Prop where
 @[default_instance]
 instance {α} (r : α → α → Prop) [Comparison r] : HComparison r r := ⟨Comparison.compare⟩
 
-@[implicit_reducible]
-def Transitive.toComparison {α} (r : α → α → Prop) [ComplementedRel r] [Transitive r] : Comparison fun x y => ¬r y x where
+theorem Transitive.toComparison {α} (r : α → α → Prop) [ComplementedRel r] [Transitive r] : Comparison fun x y => ¬r y x where
   compare := by
     intro x y nxy z
     by_cases r z x using Complemented with
@@ -223,8 +220,7 @@ class Connex {α} (r : α → α → Prop) : Prop where
 @[default_instance]
 instance {α} (r : α → α → Prop) [Connex r] : HConnex r (.≠.) := ⟨Connex.connex⟩
 
-@[implicit_reducible]
-def Connex.toAntisymmetric {α} (r : α → α → Prop) [StableEq α] [Connex r] : Antisymmetric fun x y => ¬r y x where
+theorem Connex.toAntisymmetric {α} (r : α → α → Prop) [StableEq α] [Connex r] : Antisymmetric fun x y => ¬r y x where
   antisymm := by
     intro x y nxy nyx
     by_contradiction
@@ -233,16 +229,14 @@ def Connex.toAntisymmetric {α} (r : α → α → Prop) [StableEq α] [Connex r
       | inl hyx => exact nyx hyx
       | inr hxy => exact nxy hxy
 
-@[implicit_reducible]
-def Antisymmetric.toConnex {α} (r : α → α → Prop) [WeaklyComplementedRel r] [Antisymmetric r] : Connex fun x y => ¬r y x where
+theorem Antisymmetric.toConnex {α} (r : α → α → Prop) [WeaklyComplementedRel r] [Antisymmetric r] : Connex fun x y => ¬r y x where
   connex := by
     intro x y hne
     apply and_deMorgan; intro ⟨hyx, hxy⟩
     apply hne
     exact Antisymmetric.antisymm hxy hyx
 
-@[implicit_reducible]
-def Connex.toComparison {α} (r : α → α → Prop) [ComplementedEq α] [Connex r] [Transitive r] : Comparison r where
+theorem Connex.toComparison {α} (r : α → α → Prop) [ComplementedEq α] [Connex r] [Transitive r] : Comparison r where
   compare := by
     intro x y hxy z
     by_cases x = z using Complemented with
