Algebra/Identities.lean
@@ -14,15 +14,15 @@ variable {α β} (hom : α → β)
 
 class HomCt : Prop where
   protected hom_ct : hom ct₁ = ct₂
-def hom_ct {ct₁ ct₂} [self : HomCt hom ct₁ ct₂] := self.hom_ct
+abbrev hom_ct {ct₁ ct₂} [self : HomCt hom ct₁ ct₂] := self.hom_ct
 
 class HomFn : Prop where
   protected hom_fn (x) : hom (fn₁ x) = fn₂ (hom x)
-def hom_fn {fn₁ fn₂} [self : HomFn hom fn₁ fn₂] := self.hom_fn
+abbrev hom_fn {fn₁ fn₂} [self : HomFn hom fn₁ fn₂] := self.hom_fn
 
 class HomOp : Prop where
   protected hom_op (x y) : hom (op₁ x y) = op₂ (hom x) (hom y)
-def hom_op {op₁ op₂} [self : HomOp hom op₁ op₂] := self.hom_op
+abbrev hom_op {op₁ op₂} [self : HomOp hom op₁ op₂] := self.hom_op
 
 end Hom
 
@@ -31,27 +31,27 @@ variable {α} (fn : α → α) (ct : outParam α) (fn' : outParam (α → α))
 
 class FnFix : Prop where
   protected fn_fix : fn ct = ct
-def fn_fix {ct} [self : FnFix fn ct] := self.fn_fix
+abbrev fn_fix {ct} [self : FnFix fn ct] := self.fn_fix
 
 class FnComm : Prop where
   protected fn_comm (x) : fn (fn' x) = fn' (fn x)
-def fn_comm {fn'} [self : FnComm fn fn'] := self.fn_comm
+abbrev fn_comm {fn'} [self : FnComm fn fn'] := self.fn_comm
 
 class FnLeftInv : Prop where
   protected fn_left_inv (x) : fn' (fn x) = x
-def fn_left_inv {fn'} [self : FnLeftInv fn fn'] := self.fn_left_inv
+abbrev fn_left_inv {fn'} [self : FnLeftInv fn fn'] := self.fn_left_inv
 
 class FnRightInv : Prop where
   protected fn_right_inv (x) : fn (fn' x) = x
-def fn_right_inv {fn'} [self : FnRightInv fn fn'] := self.fn_right_inv
+abbrev fn_right_inv {fn'} [self : FnRightInv fn fn'] := self.fn_right_inv
 
 class FnIdem : Prop where
   protected fn_idem (x) : fn (fn x) = fn x
-def fn_idem [self : FnIdem fn] := self.fn_idem
+abbrev fn_idem [self : FnIdem fn] := self.fn_idem
 
 class FnInvol : Prop where
   protected fn_invol (x) : fn (fn x) = x
-def fn_invol [self : FnInvol fn] := self.fn_invol
+abbrev fn_invol [self : FnInvol fn] := self.fn_invol
 
 end Fn
 
@@ -65,63 +65,63 @@ local notation "e" => id
 
 class OpAssoc : Prop where
   protected op_assoc (x y z) : (x ⋆ y) ⋆ z = x ⋆ (y ⋆ z)
-def op_assoc [self : OpAssoc op] := self.op_assoc
+abbrev op_assoc [self : OpAssoc op] := self.op_assoc
 
 class OpComm : Prop where
   protected op_comm (x y) : x ⋆ y = y ⋆ x
-def op_comm [self : OpComm op] := self.op_comm
+abbrev op_comm [self : OpComm op] := self.op_comm
 
 class OpLeftComm : Prop where
   protected op_left_comm (x y z) : x ⋆ (y ⋆ z) = y ⋆ (x ⋆ z)
-def op_left_comm [self : OpLeftComm op] := self.op_left_comm
+abbrev op_left_comm [self : OpLeftComm op] := self.op_left_comm
 
 class OpRightComm : Prop where
   protected op_right_comm (x y z) : (x ⋆ y) ⋆ z = (x ⋆ z) ⋆ y
-def op_right_comm [self : OpRightComm op] := self.op_right_comm
+abbrev op_right_comm [self : OpRightComm op] := self.op_right_comm
 
 class OpCrossComm : Prop where
   protected op_cross_comm (x₁ x₂ y₁ y₂) : (x₁ ⋆ x₂) ⋆ (y₁ ⋆ y₂) = (x₁ ⋆ y₁) ⋆ (x₂ ⋆ y₂)
-def op_cross_comm [self : OpCrossComm op] := self.op_cross_comm
+abbrev op_cross_comm [self : OpCrossComm op] := self.op_cross_comm
 
 class OpLeftId : Prop where
   protected op_left_id (x) : e ⋆ x = x
-def op_left_id {id} [self : OpLeftId op id] := self.op_left_id
+abbrev op_left_id {id} [self : OpLeftId op id] := self.op_left_id
 
 class OpRightId : Prop where
   protected op_right_id (x) : x ⋆ e = x
-def op_right_id {id} [self : OpRightId op id] := self.op_right_id
+abbrev op_right_id {id} [self : OpRightId op id] := self.op_right_id
 
 class OpLeftInv : Prop where
   protected op_left_inv (x) : x⁻¹ ⋆ x = e
-def op_left_inv {inv id} [self : OpLeftInv op inv id] := self.op_left_inv
+abbrev op_left_inv {inv id} [self : OpLeftInv op inv id] := self.op_left_inv
 
 class OpRightInv : Prop where
   protected op_right_inv (x) : x ⋆ x⁻¹ = e
-def op_right_inv {inv id} [self : OpRightInv op inv id] := self.op_right_inv
+abbrev op_right_inv {inv id} [self : OpRightInv op inv id] := self.op_right_inv
 
 class OpLeftNil : Prop where
   protected op_left_nil (x) : nil ⋆ x = nil
-def op_left_nil {nil} [self : OpLeftNil op nil] := self.op_left_nil
+abbrev op_left_nil {nil} [self : OpLeftNil op nil] := self.op_left_nil
 
 class OpRightNil : Prop where
   protected op_right_nil (x) : x ⋆ nil = nil
-def op_right_nil {nil} [self : OpRightNil op nil] := self.op_right_nil
+abbrev op_right_nil {nil} [self : OpRightNil op nil] := self.op_right_nil
 
 class OpLeftCancel : Prop where
   protected op_left_cancel (x) {y z} : x ⋆ y = x ⋆ z → y = z
-def op_left_cancel [self : OpLeftCancel op] := self.op_left_cancel
+abbrev op_left_cancel [self : OpLeftCancel op] := self.op_left_cancel
 
 class OpRightCancel : Prop where
   protected op_right_cancel (x) {y z} : y ⋆ x = z ⋆ x → y = z
-def op_right_cancel [self : OpRightCancel op] := self.op_right_cancel
+abbrev op_right_cancel [self : OpRightCancel op] := self.op_right_cancel
 
 class OpLeftDistrib : Prop where
   protected op_left_distrib (x y z) : x ⋆ (y ⊹ z) = x ⋆ y ⊹ x ⋆ z
-def op_left_distrib {op'} [self : OpLeftDistrib op op'] := self.op_left_distrib
+abbrev op_left_distrib {op'} [self : OpLeftDistrib op op'] := self.op_left_distrib
 
 class OpRightDistrib : Prop where
   protected op_right_distrib (x y z) : (x ⊹ y) ⋆ z = x ⋆ z ⊹ y ⋆ z
-def op_right_distrib {op'} [self : OpRightDistrib op op'] := self.op_right_distrib
+abbrev op_right_distrib {op'} [self : OpRightDistrib op op'] := self.op_right_distrib
 
 end Op
 
@@ -163,19 +163,19 @@ variable {α} (inv : α → α) (op : outParam (α → α → α)) (id : outPara
 
 class InvOp : Prop where
   protected inv_op (x y) : inv (op x y) = op (inv y) (inv x)
-def inv_op {op} [self : InvOp inv op] := self.inv_op
+abbrev inv_op {op} [self : InvOp inv op] := self.inv_op
 
 class InvHom : Prop where
   protected inv_hom (x y) : inv (op x y) = op (inv x) (inv y)
-def inv_hom {op} [self : InvHom inv op] := self.inv_hom
+abbrev inv_hom {op} [self : InvHom inv op] := self.inv_hom
 
 class InvInvol : Prop where
   protected inv_invol (x) : inv (inv x) = x
-def inv_invol [self : InvInvol inv] := self.inv_invol
+abbrev inv_invol [self : InvInvol inv] := self.inv_invol
 
 class InvId : Prop where
   protected inv_id : inv id = id
-def inv_id {id} [self : InvId inv id] := self.inv_id
+abbrev inv_id {id} [self : InvId inv id] := self.inv_id
 
 end Inv
 
@@ -184,15 +184,15 @@ variable {α} {β : α → α → Sort _} (inv : {{a b : α}} → β a b → β 
 
 class DInvOp : Prop where
   protected dinv_op {{a b c}} (x : β a b) (y : β c a) : inv (op x y) = op (inv y) (inv x)
-def dinv_op {op} [self : DInvOp inv op] := self.dinv_op
+abbrev dinv_op {op} [self : DInvOp inv op] := self.dinv_op
 
 class DInvInvol : Prop where
   protected dinv_invol {{a b}} (x : β a b) : inv (inv x) = x
-def dinv_invol [self : DInvInvol inv] := self.dinv_invol
+abbrev dinv_invol [self : DInvInvol inv] := self.dinv_invol
 
 class DInvId : Prop where
   protected dinv_id {{a}} : inv (id : β a a) = id
-def dinv_id {id : {a : α} → β a a} [self : DInvId inv id] := self.dinv_id
+abbrev dinv_id {id : {a : α} → β a a} [self : DInvId inv id] := self.dinv_id
 
 end DInv
 
