Algebra/Theories/Monoid.lean
@@ -16,8 +16,7 @@ class Monoid : Prop extends Semigroup (no_index s.toSemigroupSig) where
   protected op_left_id (x) : e ⋆ x = x
   protected op_right_id (x) : x ⋆ e = x
 
-@[implicit_reducible]
-protected def Monoid.infer [OpAssoc s.op] [OpLeftId s.op s.id] [OpRightId s.op s.id] : Monoid s where
+protected abbrev Monoid.infer [OpAssoc s.op] [OpLeftId s.op s.id] [OpRightId s.op s.id] : Monoid s where
   op_assoc := op_assoc _
   op_left_id := op_left_id _
   op_right_id := op_right_id _
@@ -38,8 +37,7 @@ end Monoid
 class CommMonoid : Prop extends CommSemigroup (no_index s.toSemigroupSig) where
   protected op_right_id (x) : x ⋆ e = x
 
-@[implicit_reducible]
-protected def CommMonoid.infer [OpAssoc s.op] [OpComm s.op] [OpRightId s.op s.id] : CommMonoid s where
+protected abbrev CommMonoid.infer [OpAssoc s.op] [OpComm s.op] [OpRightId s.op s.id] : CommMonoid s where
   op_assoc := op_assoc _
   op_comm := op_comm _
   op_right_id := op_right_id _
@@ -60,8 +58,7 @@ end CommMonoid
 
 class CancelMonoid : Prop extends Monoid s, CancelSemigroup (no_index s.toSemigroupSig)
 
-@[implicit_reducible]
-protected def CancelMonoid.infer [OpAssoc s.op] [OpLeftId s.op s.id] [OpRightId s.op s.id] [OpLeftCancel s.op] [OpRightCancel s.op] : CancelMonoid s where
+protected abbrev CancelMonoid.infer [OpAssoc s.op] [OpLeftId s.op s.id] [OpRightId s.op s.id] [OpLeftCancel s.op] [OpRightCancel s.op] : CancelMonoid s where
   op_assoc := op_assoc _
   op_left_id := op_left_id _
   op_right_id := op_right_id _
@@ -80,8 +77,7 @@ end CancelMonoid
 
 class CancelCommMonoid : Prop extends CommMonoid s, CancelCommSemigroup (no_index s.toSemigroupSig)
 
-@[implicit_reducible]
-protected def CancelCommMonoid.infer [OpAssoc s.op] [OpComm s.op] [OpRightId s.op s.id] [OpRightCancel s.op] : CancelCommMonoid s where
+protected abbrev CancelCommMonoid.infer [OpAssoc s.op] [OpComm s.op] [OpRightId s.op s.id] [OpRightCancel s.op] : CancelCommMonoid s where
   op_assoc := op_assoc _
   op_comm := op_comm _
   op_right_id := op_right_id _
